Messing with the write stuff, saving

scrap.v
@@ -3,763 +3,393 @@ From Coq Require Import Bool.Bool Init.Nat Arith.Arith Arith.EqNat
      Init.Datatypes Lists.List Strings.String Program.
 Require Export Coq.Strings.String.
 From mathcomp Require Import ssreflect ssrfun ssrbool eqtype.
+From TLC Require Import LibTactics LibLogic.
 Import ListNotations.
-(*setting up*)
+From Semantics Require Import programs semantics algorithms lemmas. (*shouldn't have to import both of these*)
+
 Open Scope list_scope.
-Fixpoint eq_lists {A: Type} (L1: list A) (L2: list A) (eq: A -> A -> Prop) :=
-        match L1, L2 with
-          nil, nil => True
-        | (w::ws), (d::ds) => (eq w d) /\ (eq_lists ws ds eq) (*considers order*)
-        | _ , _ => False end.
-
-Definition prefix {A: Type} (O1: list A) (O2: list A) :=
-  exists(l: nat), O1 = firstn l O2.
-
-Close Scope list_scope.
-
-Open Scope string_scope.
-Lemma eqnat: Equality.axiom Init.Nat.eqb.
-Proof.
-  unfold Equality.axiom. intros.
-  destruct (Init.Nat.eqb (x) (y)) eqn:beq.
-  - constructor. apply beq_nat_true in beq. assumption.
-  -  constructor. apply beq_nat_false in beq. assumption.
-Qed.
-Canonical nat_eqMixin := EqMixin eqnat.
-Canonical nat_eqtype := Eval hnf in EqType nat nat_eqMixin.
-(*---*)
-
-(*setting up strings equality type*)
-(* eqb_string and
-eqb_string_true_iff taken from software foundations*)
-Definition eqb_string (x y : string) : bool :=
-  if string_dec x y then true else false.
-
-Lemma eqb_string_true_iff : forall x y : string,
-    eqb_string x y = true <-> x = y.
-Proof.
-   intros x y.
-   unfold eqb_string.
-   destruct (string_dec x y) as [H |Hs].
-   - subst. split. reflexivity. reflexivity.
-   - split.
-     + intros contra. discriminate contra.
-     + intros H. rewrite H in Hs *. destruct Hs. reflexivity.
-Qed.
-(*what is the star*)
-Lemma eqstring: Equality.axiom eqb_string.
-Proof.
-  unfold Equality.axiom. intros.
-  destruct (eqb_string x y) eqn:beq.
-  - constructor. apply eqb_string_true_iff in beq. assumption.
-  -  constructor. intros contra. apply eqb_string_true_iff in contra.
-     rewrite contra in beq. discriminate beq.
-Qed.
-Canonical string_eqMixin := EqMixin eqstring.
-Canonical string_eqtype := Eval hnf in EqType string string_eqMixin.
-Close Scope string_scope.
-(***)
-
-
-(*Now, to business! Below is syntax*)
 Open Scope type_scope.
 
-Inductive boptype :=
-  Plus
-| Sub
-| Mult
-| Div
-| Mod
-| Or
-| And.
-
-(*shortcut!*)
-Inductive value :=
-    Nat (n: nat)
-  | Bool (b: bool)
-  | error. 
-Coercion Bool : bool >-> value.
-Coercion Nat : nat >-> value.
-
-(*evaluation rules for binary operations*)
-
-Fixpoint bopeval (bop: boptype) (v1 v2 :value): (value) :=
-  match bop with
-   Plus => 
-    (
-      match v1, v2 with
-        (Nat n1), (Nat n2) => Nat (add n1 n2)
-        | _, _ => error
-        end
-    )
-  | Sub => 
-    (
-      match v1, v2 with
-       (Nat n1), (Nat n2) => Nat (n1 - n2)
-        | _, _ => error
-        end
-    )
-  | Mult => 
-    (
-      match v1, v2 with
-       (Nat n1), (Nat n2) => Nat (mul n1 n2)
-        | _, _ => error
-        end
-    )
-  | Div =>
-    (
-      match v1, v2 with
-       (Nat n1), (Nat n2) =>
-                    ( if (n2 == 0) then error
-                      else Nat (n1 / n2))
-        | _, _ => error
-        end
-    )
-  | Mod =>
-    (
-      match v1, v2 with
-       (Nat n1), (Nat n2) =>
-                    ( if (n2 == 0) then error
-                     else Nat (n1 mod n2))
-        | _, _ => error
-        end
-    )
-  | Or =>
-  (
-      match v1, v2 with
-        (Bool b1), (Bool b2) => Bool (orb b1 b2)
-        | _, _ => error
-        end
-    )
-  | And =>
-  (
-      match v1, v2 with
-        (Bool b1), (Bool b2) => Bool (andb b1 b2)
-        | _, _ => error
-        end
-  )
-  end.
-
-(*value helper functions*)
-Definition isvaluable (v: value) :=
-  match v with
-    error => False
-  | _ => True
-  end.
-
-Definition isvalidbop (bop: boptype) (v1 v2 : value) :=
-  match (bopeval bop v1 v2) with
-    error => False
-  | _ => True
-   end.
-
-Definition eqb_value (x y: value) :=
-  match x, y with
-    Nat nx, Nat ny => nx == ny
-  | Bool bx, Bool byy => eqb bx byy
-  | _, _ => false
-  end.
-Definition eq_value (x y: value) := is_true(eqb_value x y).
-
-Definition eq_valueop (x y : option value) :=
-  match x, y with
-    Error, None => True
-  | Some x1, Some y1 => eq_value x1 y1
-  | _, _ => False
-  end.
-
-(*memory maps...used for both memories and checkpoints*)
-Definition map (A: Type) (eqba: A -> A -> bool):= A -> value.
-
-(*memory helpers*)
-Definition emptymap A eqba :(map A eqba) := (fun _ => error).
-Definition updatemap {A} {eqba} (m: map A eqba) (i: A) (v: value) : map A eqba := (fun j =>
-                                                               if (eqba j i) then v
-                                                               else (m j)).
-Notation "i '|->' v ';' m" := (updatemap m i v)
-  (at level 100, v at next level, right associativity).
-(*in (m1 U! m2), m1 is checked first, then m2*)
-
-Definition indomain {A} {eqba} (m: map A eqba) (x: A) :=
-  match m x with
-    error => False
-  | _ => True
-  end.
-(*this function is NOT used to check the domain of checkpoint maps.
- In particular, because an entire array can be checkpointed even if only
- one element has been assigned to (while the other elements may, in theory, still be unassigned),
-(in particular, I refer to D-WAR-CP-Arr)
-this function would return that assigned array elements are in the domain of N, while the unassigned array
-elements are not, even though both have been checkpointed.
- I resolved this problem by defining indomain_nvm, used for checkpoint maps in algorithms.v, which
-checks if a warvar is in the domain, rather than checking a location.
- *)
-(******************************************************************************************)
-
-(*******************************more syntax**********************************************)
-Inductive array :=
-  Array (s: string) (l: nat).
-
-
-Inductive volatility :=
-  nonvol
- | vol.
-
-Inductive exp :=
-  Var (s: string) (q: volatility) 
-| Val (v: value)
-| Bop (bop: boptype) (e1: exp) (e2: exp) 
-| El (a: array) (e: exp).
-Coercion Val : value >-> exp.
-Notation "a '[[' e ']]'" := (El (a) (e))
-                            (at level 100, right associativity).
-(*used subtypes to enforce the fact that only some expressions are
- memory locations*)
-(*also made the write after read type easier*)
-Definition smallvarpred := (fun x=> match x with
-                                        Var _ _ => true
-                                        | _ => false
-                                 end).
-Definition elpred  := (fun x=> match x with
-                                        El (Array _ length) (Val (Nat i)) => (i <? length)
-                                        | _ => false
-                                 end).
-(*note elpred checks if index is a natural in bounds*)
-Notation smallvar := {x: exp | smallvarpred x}.
-Notation el := {x: exp| elpred x}.
-Definition loc := smallvar + el. (*memory location type*)
-
-Definition warvar := smallvar + array. (*write after read variable type*)
-Notation warvars := (list warvar).
-(*Coercion (inl smallvar el): smallvar >-> loc.*)
-(*Coercion inl: smallvar >-> loc.*)
-
-(**location and warvar helper functions*)
-(**no need to work directly with the subtypes or sumtypes, just use these**)
-(**Note: some of these are currently unused due to implementation changes, but I left them
- as they might be useful later*)
-
-(*array and el functions*)
-
-(*checks name and length*)
-Open Scope list_scope.
-Definition eqb_array (a1 a2: array) :=
-  match a1, a2 with
-    Array s1 l1, Array s2 l2 => andb (s1 == s2) (l1 == l2)
-    end.
-Program Definition getarray (x: el): array :=
-  match val x with
-    El (arr) _ => arr
-  | _ => !
-  end.
-Next Obligation. destruct (x) as [s| | |];
-                 try (simpl in H0; discriminate H0).
-     apply (H a e). reflexivity.
+(*lemmas for the lemmas; not in paper*)
+Lemma sub_disclude: forall(N0 N1 N2: nvmem) (l: loc),
+                     subset_nvm N0 N1 ->
+                     subset_nvm N0 N2 ->
+                     not ((getmap N1) l = (getmap N2) l)
+                     -> not (In (loc_warvar l) (getdomain N0)).
+Proof. intros. intros contra. unfold subset_nvm in H. destruct H.
+       remember contra as contra1. clear Heqcontra1.
+       apply H2 in contra.
+       unfold subset_nvm in H0. destruct H0. apply H3 in contra1.
+       symmetry in contra.
+       apply (eq_trans _ _ _ contra) in contra1.
+       apply H1. assumption.
 Qed.
 
-Program Definition getindexel (x: el): value  :=
-  match val x with
-    El _ (Val v) => v
-  | _ => !
-  end.
-Next Obligation. destruct (x) as [s| | |];
-                 try (simpl in H0; discriminate H0).
-                 destruct a eqn: adestruct.
-                 destruct e;
-                 try (simpl in H0; discriminate H0).
-                 apply (H a v). subst. reflexivity.
+(*Lemma accwt_assoc_wt: forall(L1 L2: list step),
+    getwt(acc_wts L1) ++ getwt(acc_wts L2) =
+    getwt (acc_wts (L1 ++ L2)).
+  intros. induction L2.
+  + simpl. repeat rewrite app_nil_r. reflexivity.
+  + destruct a as [blah W]. simpl. *)
+
+Lemma wt_subst_fstwt: forall{L: list step} {C1 C2: context}
+  {W: the_write_stuff},
+    trace_c L C1 C2 W ->
+    incl (getfstwt W) (getwt W).
+Proof. intros L C1 C2 W T. induction T.
+       + simpl. apply (incl_refl []).
+       + induction c; try (simpl; apply (incl_refl [])); try 
+         (rewrite (lock remove) /= -lock;
+          apply remove_subst).
+       - assumption.
+       - apply (incl_app_dbl IHT1
+                                    (incl_tran
+                                    (remove_subst _ _ _)
+                                    IHT2)).
 Qed.
 
-Definition samearray_b (element: el) (a: array) := (*checks if element indexes into a*)
-  eqb_array (getarray element) a.
+(*actual lemmas*)
 
-Definition samearray (element: el) (a: array) := is_true(samearray_b element a).
-
-Definition el_arrayind_eq (e: el) (a: array) (vindex: value) := (*transitions from el type
-                                                          to a[i] representation*)
-  (samearray e a) /\ (eq_value (getindexel e) vindex).
-
-(*smallvar functions*)
-Definition isNV_b (x: smallvar) := (*checks if x is stored in nonvolatile memory*)
-  match (val x) with
-    Var _ nonvol => true
-  | _ => false
-  end.
-
-Definition isV_b (x: smallvar) :=(*checks if x is stored in volatile memory*)
-  match (val x) with
-    Var _ vol => true
-  | _ => false
-  end.
-
-Definition isNV x := is_true(isNV_b x). (*prop version of isNV_b*)
-
-Definition isV x := is_true(isV_b x). (*prop version of isV_b*)
-
-Definition samevolatility_b (x y: smallvar) := (*used for defining equality of memory locations*)
-  match isNV_b(x), isNV_b(y) with
-    true, true => true
-  | false, false => true
-  | _, _ => false
-  end.
-
-Program Definition getstringsv (x: smallvar): string :=
-  match val x with
-    Var s _ => s
-  | _ => !
-  end. 
-Next Obligation.
-    destruct x as [s| | |];
-      try (simpl in H0; discriminate H0). apply (H s q). reflexivity.
+Lemma onePointone: forall(N N' W W' R R': warvars) (l: instruction),
+    DINO_ins N W R l N' W' R' -> incl N N'.
+Proof. intros. induction H; try((try apply incl_tl); apply (incl_refl N)).
 Qed.
 
-Definition eqb_smallvar (x y: smallvar): bool :=
-  andb ((getstringsv x)==(getstringsv y)) (samevolatility_b x y).
 
-(*loc and warvar functions*)
-Definition eqb_warvar (w1 w2: warvar) :=
-  match w1, w2 with
-               inl x, inl y => eqb_smallvar x y
-             | inr x, inr y => eqb_array x y
-             | _, _ => false
-  end.
+Lemma onePointtwo: forall(N N' W R: warvars) (c c': command),
+    DINO N W R c c' N' -> incl N N'.
+Proof. intros. induction H; try(apply onePointone in H); try apply (incl_refl N); try assumption.
+       -  apply (incl_tran H IHDINO).
+       - apply (incl_appl N2 IHDINO1). (*why is coq too stupid to figure out these instantiations*)
+ Qed.
 
-Definition eq_warvar (w1 w2: warvar) :=
-  is_true (eqb_warvar w1 w2).
-
-(*checks if w was recorded as read/written to in warvar list W*)
-Fixpoint memberwv_wv_b (input: warvar) (w: warvars) :=
-  match w with
-    [] => false
-  | wv::wvs => orb (eqb_warvar input wv) (memberwv_wv_b input wvs) 
-end.
-
-Definition memberwv_wv (w: warvar) (W: warvars) := is_true(memberwv_wv_b w W).
+Lemma Two: forall(N N' W W' R R' N1: warvars) (l: instruction),
+    DINO_ins N W R l N' W' R' -> incl N' N1 -> WAR_ins N1 W R l W' R'.
+  intros. induction H; try (constructor; assumption || (apply War_noRd; assumption));
+            (apply WAR_Checkpointed || apply WAR_Checkpointed_Arr);
+            (repeat assumption); apply H0; unfold In; left; reflexivity.
+Qed.
 
 
-Definition eqb_loc (l1: loc) (l2: loc) :=
-  match l1, l2 with
-    inl x, inl y => eqb_smallvar x y
-  | inr x, inr y => andb (eqb_array (getarray x) (getarray y))
-                        (eqb_value (getindexel x) (getindexel y))
-  | _, _ => false 
-  end. (*might be nice to have values as an equality type here*)
-
-(*converts a location to a warvar*)
-Fixpoint loc_warvar (l: loc) : warvar := 
-  match l with
-    inl x => inl x
-  | inr el => inr (getarray el)
-  end.
-
-(*checks if a location input has been stored as a WAR location in w*)
-Definition memberloc_wvs_b (input: loc) (w: warvars) :=
-  memberwv_wv_b (loc_warvar input) w.
-(*******************************************************************)
-
-(*more syntax*)
-Inductive instruction :=
-  skip
-| asgn_sv (x: smallvar) (e: exp) (*could distinguish between NV and V assignments as well here*)
-| asgn_arr (a: array) (i: exp) (e: exp) (*i is index, e is new value of a[i]*)
-| incheckpoint (w: warvars)
-| inreboot.
-(*added the in prefixes to distinguish from the observation reboots
- and checkpoints*)
-
-Inductive command :=
-  Instruct (l: instruction)
-| Seqcom (l: instruction) (c: command) (*added suffix to distinguish from Seq ceval
-                                         constructor*)
-| ite (e: exp) (c1: command) (c2: command).
-
-Notation "l ';;' c" := (Seqcom l c)
-                         (at level 100).
-
-Notation "'TEST' e 'THEN' c1 'ELSE' c2 " := (ite e c1 c2)
-                                              (at level 100).
-Coercion Instruct : instruction >-> command.
-(*******************************************************************)
-
-(******setting up location equality relation for memory maps******************)
-(****************************************************************)
-
-(****************************memory*************************************)
-
-(*memory locations defined above warvars*)
-Notation mem := (map loc eqb_loc). (*memory mapping*)
-
-Inductive nvmem := (*nonvolatile memory*)
-  NonVol (m : mem) (D: warvars). (*extra argument to keep track of checkpointed warvars because
-                                  it might be nice to have for when we do checkpoint proofs*)
-
-Inductive vmem := (*volatile memory*)
-  Vol (m : mem).
-
-(*I could change nvmem and vmem to enforce that they only take in smallvars
- of the correct type but it's already checked in my evaluation rules*)
-
-(**************************helpers for the memory maps*********************************************)
-
-(*note: a lot of these aren't being used right now because, after I changed the types
- of DINO and WAR, they aren't necessary.
- I won't delete them because having the domain of the checkpoint easily accessible and
- manipulable could be handy in the future*)
-
-Definition getmap (N: nvmem) :=
-  match N with NonVol m _ => m end.
-
-Definition getdomain (N: nvmem) :=
-  match N with NonVol _ D => D end.
-
-Definition getvalue (N: nvmem) (i: loc) :=
-  (getmap N) i.
-  Notation "v '<-' N" := (getvalue N v)
-                           (at level 40).
+Theorem DINO_WAR_correct: forall(N W R N': warvars) (c c': command),
+    DINO N W R c c' N' -> (forall(N1: warvars), incl N' N1 -> WARok N1 W R c').
+  intros N W R c c' N' H. induction H; intros N0 Hincl.
+  - eapply WAR_I. applys Two H Hincl.
+  - eapply WAR_Seq. applys Two H. apply onePointtwo in H0. eauto using incl_tran.
+    apply (IHDINO N0 Hincl).
+  - eapply WAR_If; (try eassumption);
+      ((apply IHDINO1; apply incl_app_l in Hincl)
+       || (apply IHDINO2; apply incl_app_r in Hincl)); assumption.
+  - intros. apply WAR_CP. apply IHDINO. apply (incl_refl N').
+Qed.
 
 
-  (*updates domain and mapping function*)
-Definition updateNV (N: nvmem) (i: loc) (v: value) :=
-  match N with NonVol m D =>
-               NonVol (updatemap m i v) (
-                        match i with 
-                          inl x => ((inl x) :: D) (*i is a smallvar*)
-                        | inr el => ((inr (getarray el))::D) (*i is an array element*)
-                                     (*here I add the entire array to the domain
-                                      even though only one element has been assigned to*)
-                        end
-                      )
-  end.
-
-(*used to update NV memory with checkpoint*)
-(*checks N first, then N'*)
-Definition updatemaps (N: nvmem) (N': nvmem): nvmem :=
-  match N, N' with
-    NonVol m D, NonVol m' D' => NonVol
-  (fun j =>
-     match m j with
-     error => m' j
-     | x => x
-     end
-  )
-  (D ++ D') (*inclusion of duplicates*)
-  end.
-Notation "m1 'U!' m2" := (updatemaps m1 m2) (at level 100).
-
-Notation emptyNV := (NonVol (emptymap loc eqb_loc) nil).
-Definition reset (V: vmem) := Vol (emptymap loc eqb_loc).
-
-(*restricts memory map m to domain w*)
-(*doesn't actually clean the unnecessary variables out of m*)
-Definition restrict (N: nvmem) (w: warvars): nvmem :=
-  match N with NonVol m D => NonVol
-    (fun input => if (memberloc_wvs_b input w) then m input else error) w  end.
-
-Notation "N '|!' w" := (restrict N w) 
-  (at level 40, left associativity).
-
-(*prop determining if every location in array a is in the domain of m*)
-Definition indomain_nvm (N: nvmem) (w: warvar) :=
-  memberwv_wv_b w (getdomain N).
-
-Definition isdomain_nvm (N: nvmem) (w: warvars) :=
-  eq_lists (getdomain N) w eq_warvar.
-
-(********************************************)
-Inductive cconf := (*continuous configuration*)
-  ContinuousConf (triple: nvmem * vmem * command).
-
-Notation context := (nvmem * vmem * command). 
-
-Inductive iconf := (*intermittent configuration*)
-  IntermittentConf (qple: context * nvmem * vmem * command).
-
-Definition ro := loc * value. (*read observation*)
-Definition readobs := list ro.
-
-Notation NoObs := ([]: readobs).
-
-Inductive obs := (*observation*)
-  Obs (r: readobs)
-| reboot
-| checkpoint.
-Coercion Obs : readobs >-> obs.
-
-Notation obseq := (list obs). (*observation sequence*)
-
-Open Scope list_scope.
-
-(*helpers for observations and warvars*)
-(*don't need the first two as there's no way to construct
- a relation instance that would violate these*)
-Definition hasCheckpt (O: obseq) := In checkpoint O.
-
-Definition isAllRead (O: obseq) := not(hasCheckpt O) /\ not(In reboot O).
-
-(*converts from list of read locations to list of
-WAR variables
- *)
-Fixpoint readobs_warvars (R: readobs) : warvars := 
-  match R with
-    nil => nil
-| (r::rs) => match r with
-              (location, _) => (*get the location r has recorded reading from*)
-              (match location with
-                inl x => (inl x)::(readobs_warvars rs) (*location is a smallvar*)
-              | inr el => (inr (getarray el))::(readobs_warvars rs) (*location is an array element
-                                                                   records entire array in warvars*)
-              end)
-           end
-  end.
-
-(*relations between continuous and intermittent traces*)
-(*Definition reduces (O1 O2: readobs) :=
-  (prefix O1 O2*)
-Notation "S <= T" := (prefix S T).
-
-(*Where
-O1 is a sequence of read observation lists,
-where each continguous read observation list is separated from those adjacent to it by a reboot,
-and O2 is a read observation list,
-prefix_seq determines if each ro list in O1 is a valid
-prefix of O2*)
-Inductive prefix_seq: obseq -> readobs -> Prop :=
-  RB_Base: forall(O: readobs), prefix_seq [Obs O] O
-| RB_Ind: forall(O1 O2: readobs) (O1': obseq),
-    O1 <= O2 -> prefix_seq O1' O2 -> prefix_seq ([Obs O1] ++ [reboot] ++ O1') O2.
-
-(* Where
-O1 is a sequence of ((read observation list sequences), where
-each continguous read observation list is separated from those adjacent to it
-by a reboot), where each sequence is separated from those adjacent to it by a checkpoint.
-ie, each read observation list in a given read observation sequence
-occurs within the same checkpointed region as all the other read observation lists in that sequence,
-O2 is a read observation list,
-prefix_frag determines if each ro list in O1 is a prefix of some FRAGMENT of O2
-(where the fragments are separated by the positioning of the checkpoints in O1)
- *)
-Inductive prefix_fragment: obseq -> readobs -> Prop :=
-  CP_Base: forall(O1: obseq) (O2: readobs), prefix_seq O1 O2 -> prefix_fragment O1 O2
-| CP_IND: forall(O1 O1': obseq) (O2 O2': readobs),
-    prefix_seq O1 O2 -> prefix_fragment O1' O2' ->
-   prefix_fragment (O1 ++ [checkpoint] ++ O1') (O2 ++ O2'). 
-
-(***************************************************************)
-
-(*traces*)
-(*The trace type contains
-1. a list of configurations, where each configuration follows from
- its leftmost neighbor by an evaluation rule
-2. a list of warvars which have been written to
-3. a list of warvars which have been read from
-4. a list of warvars which have been written to before they have been read from
- *)
-
-Inductive trace_c: list cconf -> warvars -> warvars -> warvars -> Prop :=
-  Empty: trace_c nil nil nil nil
-| 
-.
-
-    (*need starting point and ending point for trace*)
-
-(****************continuous operational semantics***********************)
-(*evaluation relation for expressions*)
-Inductive eeval: nvmem -> vmem -> exp -> readobs -> value -> Prop :=
-  VAL: forall(N: nvmem) (V: vmem) (v: value),
-    (isvaluable v) -> (*extra premise to check if v is valuable*)
-    eeval N V v NoObs v
-| BINOP: forall(N: nvmem) (V: vmem)
-          (e1: exp) (e2: exp)
-          (r1: readobs) (r2: readobs)
-          (v1: value) (v2: value) (bop: boptype),
-    eeval N V e1 r1 v1 ->
-    eeval N V e2 r2 v2 -> 
-    (isvalidbop bop v1 v2) -> (*extra premise to check if v1, v2, bop v1 v2 valuable*)
-    eeval N V (Bop bop e1 e2) (r1++ r2) (bopeval bop v1 v2)
-| RD_VAR_NV: forall(N: nvmem) (mapV: vmem) (x: smallvar) (v: value),
-    eq_value ((inl x) <-N) v ->
-    isNV(x) -> (*extra premise to make sure x is correct type for NV memory*)
-    (isvaluable v) -> (*extra premise to check if v is valuable*)
-    eeval N mapV (val x) [((inl x), v)] v
-| RD_VAR_V: forall(N: nvmem) (mapV: mem) (x: smallvar) (v: value),
-    eq_value (mapV (inl x)) v ->
-    isV(x) -> (*extra premise to make sure x is correct type for V memory*)
-    (isvaluable v) -> (*extra premise to check if v is valuable*)
-    eeval N (Vol mapV) (val x) [((inl x), v)] v
-| RD_ARR: forall(N: nvmem) (V: vmem)
-           (a: array)
-           (index: exp)
-           (rindex: readobs)
-           (vindex: value)
-           (element: el)
-           (v: value),
-    eeval N V (index) rindex vindex ->
-    eq_value ((inr element) <-N) v ->
-    (el_arrayind_eq element a vindex) -> (*extra premise to check that inr element
-                                        is actually a[vindex] *)
-(*well-typedness, valuability, inboundedness of vindex are checked in elpred*)
-    (isvaluable v) -> (*extra premise to check if v is valuable*)
-    eeval N V (a[[index]]) (rindex++[((inr element), v)]) v
-.
-(*ask Arthur why this notation doesn't work *)
-
-(*Reserved Notation "'{'N V'}=[' e ']=> <'r'>' v" (at level 40).
-Inductive eevaltest: nvmem -> vmem -> exp -> obs -> value -> Prop :=
-  VAL: forall(N: nvmem) (V: vmem) (v: value), 
-    {N V} =[ v ]=> <reboot> v
-  where "{N V}=[ e ]=> <r> v" := (eevaltest N V e r v).*)
-
-(****************************************************************************)
-
-(**********continuous execution semantics*************************)
+Lemma eight: forall(N0 N1 N2: nvmem) (V0: vmem) (c0: command),
+              (subset_nvm N0 N1) ->
+              (subset_nvm N0 N2) ->
+              current_init_pt N0 V0 c0 N1 N2 ->
+              same_pt N1 V0 c0 c0 N1 N2.
+Proof. intros. inversion H1; subst.
+       apply (same_mem (CTrace_Empty (N1, V0, c0))
+                       T); (try assumption).
+       - simpl. intros contra. contradiction.
+       - intros. simpl.
+         assert (H6: not (In (loc_warvar l) (getdomain N0))) by
+               apply (sub_disclude N0 N1 N2 l H H0 H5).
+           apply H4 in H5. destruct H5. split. 
+         + unfold Wt. apply ((wt_subst_fstwt T) l H5).
+         + split.
+             - unfold remove. unfold in_loc_b. rewrite filter_false.
+                 apply H5.
+             - intros contra. contradiction.
+         + apply H6 in H5. contradiction.
+Qed.
 
 
-(*evaluation relation for commands*)
-Inductive cceval: nvmem -> vmem -> command -> obseq -> nvmem -> vmem -> command -> Prop :=
-  NV_Assign: forall(x: smallvar) (N: nvmem) (V: vmem) (e: exp) (r: readobs) (v: value),
-    eeval N V e r v ->
-    isNV(x) -> (*checks x is correct type for NV memory*)
-    (isvaluable v) -> (*extra premise to check if v is valuable*)
-    cceval N V (asgn_sv x e) [Obs r]
-           (updateNV N (inl x) v) V skip
-| V_Assign: forall(x: smallvar) (N: nvmem) (mapV: mem) (e: exp) (r: readobs) (v: value),
-    eeval N (Vol mapV) e r v ->
-    isV(x) -> (*checks x is correct type for V memory*)
-    (isvaluable v) -> (*extra premise to check if v is valuable*)
-    cceval N (Vol mapV) (asgn_sv x e) [Obs r] N (Vol ((inl x) |-> v ; mapV)) skip
-| Assign_Arr: forall (N: nvmem) (V: vmem)
-               (a: array)
-               (ei: exp)
-               (ri: readobs)
-               (vi: value)
-               (e: exp)
-               (r: readobs)
-               (v: value)
-               (element: el),
-    eeval N V ei ri vi ->
-    eeval N V e r v ->
-    (el_arrayind_eq element a vi) -> (*extra premise to check that inr element
-                                        is actually a[vindex] *)
-(*well-typedness, valuability, inboundedness of vindex are checked in elpred*)
-    (isvaluable v) -> (*extra premise to check if v is valuable*)
-    cceval N V (asgn_arr a ei e) [Obs (ri++r)]
-           (updateNV N (inr element) v) V skip
-    (*valuability and inboundedness of vindex are checked in sameindex*)
-| CheckPoint: forall(N: nvmem)
-               (V: vmem)
-               (c: command)
-               (w: warvars),
-               cceval N V ((incheckpoint w);; c) [checkpoint]
-               N V c
-| Skip: forall(N: nvmem)
-         (V: vmem)
-         (c: command),
-    cceval N V (skip;;c) [Obs NoObs] N V c
-| Seq: forall (N: nvmem)
-         (N': nvmem)
-         (V: vmem)
-         (V': vmem)
-         (l: instruction)
-         (c: command)
-         (o: obs),
-    cceval N V l [o] N' V' skip ->
-    cceval N V (l;;c) [o] N' V' c
-| If_T: forall(N: nvmem)
-         (V: vmem)
-         (e: exp)
-         (r: readobs)
-         (c1: command)
-         (c2: command),
-    eeval N V e r true -> 
-    cceval N V (TEST e THEN c1 ELSE c2) [Obs r] N V c1
-| If_F: forall(N: nvmem)
-         (V: vmem)
-         (e: exp)
-         (r: readobs)
-         (c1: command)
-         (c2: command),
-    eeval N V e r false ->
-    cceval N V (TEST e THEN c1 ELSE c2) [Obs r] N V c2.
+Ltac destruct3 zero one two three:= destruct zero as [Annoying one]; destruct Annoying as [two three].
 
-(************************************************************)
+Ltac ex_destruct3 H := destruct H as [var1 Annoying]; destruct Annoying as [var2 Annoying1];
+                       destruct Annoying1 as [var3 H].
 
-(**********intermittent execution semantics*************************)
-(*evaluation relation for commands*)
-Inductive iceval: context-> nvmem -> vmem -> command -> obseq -> context -> nvmem -> vmem -> command -> Prop :=
-  CP_PowerFail: forall(k: context) (N: nvmem) (V: vmem) (c: command),
-                 iceval k N V c
-                        nil
-                        k N (reset V) inreboot
- | CP_CheckPoint: forall(k: context) (N: nvmem) (V: vmem) (c: command) (w: warvars),
-                 iceval k N V ((incheckpoint w);;c)
-                        [checkpoint]
-                        ((N |! w), V, c) N V c 
- | CP_Reboot: forall(N: nvmem) (N': nvmem)(*see below*) (*N is the checkpointed one*)
-               (V: vmem) (V': vmem)
-               (c: command), 
-     iceval (N, V, c) N' V' inreboot
-            [reboot]
-            (N, V, c) (N U! N') V c
- | CP_NV_Assign: forall(k: context) (x: smallvar) (N: nvmem) (V: vmem) (e: exp) (r: readobs) (v: value),
-    eeval N V e r v ->
-    isNV(x) -> (*checks x is correct type for NV memory*)
-    (isvaluable v) -> (*extra premise to check if v is valuable*)
-    iceval k N V (asgn_sv x e)
-           [Obs r]
-           k (updateNV N (inl x) v) V skip
-| CP_V_Assign: forall(k: context) (x: smallvar) (N: nvmem) (mapV: mem) (e: exp) (r: readobs) (v: value),
-    eeval N (Vol mapV) e r v ->
-    isV(x) -> (*checks x is correct type for V memory*)
-    (isvaluable v) -> (*extra premise to check if v is valuable*)
-    iceval k N (Vol mapV) (asgn_sv x e)
-           [Obs r]
-           k N (Vol ((inl x) |-> v ; mapV)) skip
-| CP_Assign_Arr: forall (k: context) (N: nvmem) (V: vmem)
-               (a: array)
-               (ei: exp)
-               (ri: readobs)
-               (vi: value)
-               (e: exp)
-               (r: readobs)
-               (v: value)
-               (element: el),
-    eeval N V ei ri vi ->
-    eeval N V e r v ->
-    (el_arrayind_eq element a vi) -> (*extra premise to check that inr element
-                                        is actually a[vindex] *)
-(*well-typedness, valuability, inboundedness of vindex are checked in elpred*)
-    (isvaluable v) -> (*extra premise to check if v is valuable*)
-    iceval k N V (asgn_arr a ei e)
-           [Obs (ri++r)]
-           k (updateNV N (inr element) v) V skip
-| CP_Skip: forall(k: context) (N: nvmem)
-         (V: vmem)
-         (c: command),
-    iceval k N V (skip;;c) [Obs NoObs] k N V c
-|CP_Seq: forall (k: context)
-         (N: nvmem) (N': nvmem)
-         (V: vmem) (V': vmem)
-         (l: instruction)
-         (c: command)
-         (o: obs),
-    iceval k N V l [o] k N' V' skip ->
-    iceval k N V (l;;c) [o] k N' V' c
-|CP_If_T: forall(k: context) (N: nvmem) (V: vmem)
-         (e: exp)
-         (r: readobs)
-         (c1: command)
-         (c2: command),
-    eeval N V e r true -> 
-    iceval k N V (TEST e THEN c1 ELSE c2) [Obs r] k N V c1
-|CP_If_F: forall(k: context) (N: nvmem) (V: vmem)
-         (e: exp)
-         (r: readobs)
-         (c1: command)
-         (c2: command),
-    eeval N V e r false ->
-    iceval k N V (TEST e THEN c1 ELSE c2) [Obs r] k N V c2.
-(*CP_Reboot: I took out the equals premise and instead built it
-into the types because I didn't want to define a context equality function*)
+Ltac destruct_ms M L WT T:= destruct M as [L neverseen]; destruct neverseen as [WT neverseen];
+                            destruct neverseen as [T M].
+
+Ltac generalize_5 N N' V V' O := generalize dependent N;
+                               generalize dependent N';
+                               generalize dependent V;
+                               generalize dependent V';
+                               generalize dependent O.
+(*Ltac get_trace M :=*)
+
+Lemma trace_stops: forall {N N': nvmem} {V V': vmem}
+                    {l: instruction} {c: command}
+  {L: list step} {W: the_write_stuff},
+    trace_c L (N, V, Ins l) (N', V', c) W ->
+    (c = Ins l) \/ (c = skip).
+Proof.
+  intros N N' V V' l c L W T. dependent induction T.
+  + constructor.
+  + reflexivity.
+  + inversion c0; subst; try(right; reflexivity).
+  + destruct3 S2 cmid nmid vmid.
+    assert (cmid = l \/ cmid = skip).
+    {
+      apply (IHT1 N nmid V vmid l cmid); reflexivity.
+    }
+  + inversion H; subst.
+       -  eapply IHT2; reflexivity.
+       - right.
+         destruct (IHT2 nmid N' vmid V' skip c); (reflexivity || assumption).
+Qed.
+
+(*Lemma observe_checkpt: forall {N N': nvmem} {V V': vmem}
+                     {c c': command} {w: warvars}
+                    {O: obseq} {W: the_write_stuff},
+    trace_c (N, V, (incheckpoint w ;; c)) (N', V', c') O W ->
+    c' = (incheckpoint w ;; c) \/ In checkpoint O.
+  intros N N' V V' c c' w O W T.
+  dependent induction T.
+  + left. reflexivity.
+  +  inversion c0; subst. right.  apply(in_eq checkpoint).
+     inversion H8.
+  + destruct3 Cmid. destruct (IHT1 N nmid V vmid c cmid w); subst; try reflexivity.
+      - destruct (IHT2 nmid N' vmid V' c c' w); subst; try reflexivity;
+          [left; reflexivity | right; apply (in_app_r H)].
+      - right. apply (in_app_l H).
+Qed.
+
+
+(*could also add that written set of c -> c2 is inside written set of
+ l;;c -> c2 but ill wait till I need it*)
+Lemma single_step_all: forall{N N2: nvmem} {V V2: vmem}
+                    {l: instruction} {c c2: command}
+                    {O: obseq} {W: the_write_stuff},
+    trace_c (N, V, l;;c) (N2, V2, c2) O W ->
+    not ((l ;;c ) = c2) -> (*empty trace case *)
+    exists(N1: nvmem) (V1: vmem) (O1: obseq), ((multi_step_c (N1, V1, c) (N2, V2, c2) O1)
+                                          /\ (incl O1 O)
+                                          ).
+  intros N N2 V V2 l c c2 O W T H. dependent induction T. 
+  + exfalso. apply H. reflexivity.
+  + inversion c0; subst; exists N2 V2 (nil : obseq); try (split;
+                                                     [exists emptysets; repeat constructor | apply empty_sub]).
+  + destruct3 Cmid. assert (Dis: (l ;; c) = cmid \/ not ((l;;c) = cmid))
+      by (apply classic). destruct Dis.
+  - subst. 
+    cut (exists N1 V1 O1, (multi_step_c (N1, V1, c) (N2, V2, c2) O1 /\ incl O1 O2)).
+    + intros H3. ex_destruct3 H3. exists var1 var2 var3. destruct H3 as [H31 H32]. split.
+      -  assumption.
+      - apply (incl_appr O1 H32).  
+   + apply (IHT2 nmid N2 vmid V2 l c c2); try reflexivity; try assumption.
+ -  assert (Hmid: exists N3 V3 O3,
+               multi_step_c (N3, V3, c) (nmid, vmid, cmid) O3
+              /\ incl O3 O1
+           ).
+     - eapply IHT1; try reflexivity; try assumption.
+       assert (Hend: multi_step_c (nmid, vmid, cmid)
+                                              (N2, V2, c2) O2
+            ).
+       + exists W2. apply (inhabits T2).
+       ex_destruct3 Hmid.
+       destruct Hmid as [Hmid Obsmid].
+     destruct_ms Hmid Tmid Wmid.
+     destruct_ms Hend Tend Wend.
+     exists var1 var2 (var3 ++ O2). split.
+     + exists (append_write Wmid Wend ). constructor.
+       apply (CTrace_App Tmid Tend).
+     +  apply (incl_app_dbl Obsmid (incl_refl O2)).
+Qed.
+
+(*hack to get around destroying conjunctions all the time*)
+Lemma single_step: forall{N N2: nvmem} {V V2: vmem}
+                    {l: instruction} {c c2: command}
+                    {O: obseq} {W: the_write_stuff},
+    trace_c (N, V, l;;c) (N2, V2, c2) O W ->
+    not ((l ;;c ) = c2) -> (*empty trace case *)
+    exists(N1: nvmem) (V1: vmem) (O1: obseq), ((multi_step_c (N1, V1, c) (N2, V2, c2) O1)
+                                         ).
+Proof. intros. pose proof (single_step_all X H).
+       ex_destruct3 H0. destruct H0.
+       exists var1 var2 var3. assumption.
+Qed.*)
+
+(*hacky extra hypothesis L = [], coq should take care of remembering that*)
+Lemma trace_stops: forall {C1 C2: context} {W: the_write_stuff}
+                     {L: list step}
+  (T: trace_c L C1 C2 W), L = [] -> C1 = C2 /\ W = emptysets.
+Proof. intros C1 C2 W L T. induction T; intros.
+       + split; reflexivity.
+       + inversion H.
+       + apply app_eq_nil in H. destruct H. destruct (IHT1 H).
+         destruct (IHT2 H0). subst. split; reflexivity.
+Qed.
+
+Lemma undo_gets: forall(W: the_write_stuff),
+    (getwt W, getrd W, getfstwt W) = W.
+  intros. destruct3 W f g h. simpl. reflexivity. Qed.
+
+  (*ask arthur what is up with the variable names where
+this doesnt work destruct3 W one two three.*)
+
+
+(*clean this one up*)
+Lemma single_step: forall {C1 C2 C3 C4: context} {W: the_write_stuff}
+                     {L: list step}
+                     {O: obseq}
+  (T: trace_c L C1 C2 W), L = [(C3, C4, O)] -> cceval_w C1 O C2 W /\ C1 = C3 /\ C2 = C4.
+Proof. intros C1 C2 C3 C4 W L a T. induction T.
+       + intros. inversion H. 
+       + intros.  inversion H. subst. split; [assumption | split; reflexivity].
+       + intros H.
+         apply app_eq_unit in H. destruct H; destruct H; subst.
+       - destruct (trace_stops T1). reflexivity. subst.
+         unfold append_write. simpl. unfold remove. unfold in_loc_b.
+         rewrite filter_false. rewrite undo_gets. apply IHT2. reflexivity.
+       - destruct (trace_stops T2). reflexivity. subst.
+         unfold append_write. simpl. repeat rewrite app_nil_r.
+         rewrite undo_gets. apply IHT1. reflexivity.
+Qed.
+
+
+(*N0 is checkpointed variables*)
+Lemma ten: forall(N0 W R: warvars) (N N': nvmem) (V V': vmem)
+            (O: obseq) (c c': command),
+            WARok N0 W R c ->
+            multi_step_c (N, V, c) (N', V', c') O ->
+            not (In checkpoint O) ->
+            exists(W' R': warvars), WARok N0 W' R' c'.
+  intros.
+  (*unfold multi_step_ic in H0. destruct H0 as [Wr].*)
+  generalize_5 N N' V V' O.
+  induction H; intros.
+  + 
+    destruct_ms H0 L Wr T.
+    generalize_5 N N' V V' O.
+    generalize dependent l.
+    generalize dependent c'.
+    induction L; intros.
+  - assert ( (N0, V, Ins l) = (N', V', c')).
+    + apply (trace_stops T). reflexivity.
+      inversion H2. subst. exists W R. eapply WAR_I. apply H.
+  - destruct L. destruct3 a Oa C1 C2.
+    remember T as T1. clear HeqT1. eapply single_step in T.
+    inversion T; subst.
+    remember T as T1. clear HeqT1. apply trace_not_empty in T. exfalso.
+    apply T. reflexivity.
+  + exists W R. applys WAR_I. apply H.
+  + inversion c; subst; try (exists W R; applys WAR_I; constructor).
+  - destruct3 Cmid. 
+    assert (Hcmid: cmid = Ins l \/ cmid = skip) by
+                                           (apply (trace_stops T1)).
+    destruct Hcmid; subst.
+  - eapply IHT2; (try reflexivity). apply H.
+    (*apply (inhabits T2).*)
+  - intros contra. eapply in_app_r in contra. apply H1 in contra. contradiction.
+ (* - apply (inhabits T2).*)
+    - apply trace_stops in T2. destruct T2; subst; exists W R;
+                                 eapply WAR_I; constructor.
+      + (*inversion H0 as [T].*)
+    destruct_ms H0 T Wr.
+        apply observe_checkpt in T. destruct T.
+        - subst. exists W R. constructor. assumption.
+        - apply H1 in H0. contradiction.
+        - assert (Dis: (l ;; c) = c' \/ not ((l;;c) = c'))
+      by (apply classic). destruct Dis.
+         + subst. exists W R. eapply WAR_Seq. apply H. assumption.
+         + 
+           (*destruct H0 as [T0].*)
+           destruct_ms H2 T0 W0.
+           pose proof (single_step_all T0 H3) as destroyme.
+           ex_destruct3 destroyme.
+           destruct destroyme as [MS sub].
+           destruct_ms MS T1 WT1.
+           eapply (IHWARok var3).
+        - intros contra. apply sub, H1 in contra. contradiction. (*cool applying!!*)
+          exists WT1. apply (inhabits T1).
+ - destruct_ms H3 T3 WT3.
+            inversion T3; subst.
+
+          apply (inhabits (single_step_all T0 H3)).
+eapply IHT2.
+          (*garbage below*)
+        inversion T; subst.
+        exists W R. constructor. assumption.
+        inversion H3; subst.
+        exfalso. apply H1. apply in_eq.
+        inversion H2.
+
+       apply (in_eq H1). in H1. discriminate H1.
+      eapply IHT2. (try reflexivity); try (apply WAR_Skip).
+     apply WAR_Skip.
+
+     
+     apply H. apply (inhabits T2).
+    intros contra. eapply or_intror in contra.
+    apply in_or_app in contra. apply H1 in contra. contradiction.
+
+
+(*garbage below*)
+    applys H1 in (in_or_app contra).
+      inversion H2. subst. eapply IHT2.
+      assert (WAR_ins N0 W R l0 W' R')
+    +
+
+    inversion T1; subst.
+    + inversion T2; subst; try (applys WAR_I; constructor).
+    + applys WAR_I. apply H.
+
+    destruct Cmid as [Annoying cmid].
+      destruct Annoying as [nmid vmid].
+      apply (IHT1 N nmid V vmid c' l).
+     - assumption.
+     - 
+      apply (inhabits T1 ).
+      
+
+    remember H as Hwarins. clear HeqHwarins. eapply (IHT1) in H. apply H.
+    destruct Cmid as [Annoying cmid]. destruct Annoying
+                                                 as [nmid vmid]. apply (inhabits T1 ).
+    inversion H0; subst.
+       - applys WAR_I. apply H.
+       - inversion H3; subst; try (applys WAR_I; constructor).
+         + inversion H0; subst. applys WAR_I. apply H.
+         + inversion H5; subst; try(applys WAR_I; constructor).
+  + subst.
+
+
+  inversion H0; subst.
+  + exists W. exists R. assumption.
+  + inversion H2. subst. inversion H3; subst; try (exists W R; applys WAR_I; constructor).
+  - induction H.
+    + inversion H2. subst. inversion H3. subst.
+  - exists W R. applys WAR_I. apply H.
+  - subst. inversion H5. subst. exists W R. applys WAR_I. constructor.
+
+
+    destruct l. constructor.
+
+    + exists W R. applys WAR_I. constructor.
+  induction H.
+  + inversion H0. subst.
+  + unfold single_com in H2.
+    induction c'.
+  - induction l.
+    + applys WAR_I.
+    applys WAR_I.
+    induction c. inversion H3; subst; exists W R; applys WAR_I; constructor.
+    (*the existence is hacky here but I can't
+                            figure out how to be smarter
+                            w instantiations*)
+    -  
+    - applys WAR_Vol.
+
+      inversion H3. subst.
+    (try (apply WAR_I); constructor).
+             eapply H. induction c'.
+    - simpl.
+
+  exists(locs_warvars (getwt Wr)). exists(locs_warvars (getrd Wr)).
+
+
 
 Close Scope list_scope.
-Close Scope type_scope.
